two_state_model/hoare.v
@@ -9,24 +9,93 @@ Require Export external_state_semantics.
 Require Export Coq.Numbers.BinNums.
 Require Export ZArith.
 
-
 Module Hoare.
 
-  Export Assert.
+  Import LanguageDefinition.
+  Import Assert.
 
-  Inductive 
+  Inductive big_step_reduction : module -> config -> config -> Prop :=
+  | bsr_single : forall M σ1 σ2, reduction M σ1 σ2 ->
+                            big_step_reduction M σ1 σ2
 
-  Definition hoare_triple (M : module)(P : asrt)(s : stmt)(Q : asrt) :=
-    forall χ lcl s' ψ σ1 σ2, reduction M (χ, frm lcl (c_stmt s') ;; ψ) σ2 ->
-                        s' = s ->
-                        σ1 = (χ, frm lcl (c_stmt s') ;; ψ) ->
-                        sat M σ1 P ->
-                        sat M σ2 Q.
+  | bsr_trans : forall M σ1 σ2 σ3, reduction M σ1 σ2 ->
+                              big_step_reduction M σ2 σ3 ->
+                              big_step_reduction M σ1 σ2.
 
-  Notation "M ⊨ ⦃ P ⦄ s ⦃ Q ⦄" := (hoare_triple M P s Q)(at level 40).
+  Definition hoare_semantics (M : module)(P : asrt)(s : stmt)(Q : asrt) :=
+    forall χ lcl c ψ χ' lcl', big_step_reduction M (χ, frm lcl (s :: nil) ;; nil) (χ', frm lcl' nil ;; nil) ->
+                         sat M (χ, frm lcl (s :: c) ;; ψ) P ->
+                         sat M (χ', frm lcl' c ;; ψ) Q.
+
+  Notation "M ⊨ ⦃ P ⦄ s ⦃ Q ⦄" := (hoare_semantics M P s Q)(at level 40).
 
   (* Proof Rules *)
 
-  Inductive hoare : module -> asrt -> stmt -> Q
+  Definition asrt_proof (M : module)(A : asrt) : Prop := forall σ, sat M σ A.
+
+  #[global] Instance exp_subst : Subst exp var exp:=
+    {
+      sbst :=
+        fix sbst' e x e' :=
+          match e with
+          | e_var y => if eqb x y
+                        then e'
+                        else e_var y
+          | e_fld e0 f => e_fld (sbst' e0 x e') f
+          | e_class e0 C => e_class (sbst' e0 x e') C
+          | e_ghost e0 g e1 => e_ghost (sbst' e0 x e') g (sbst' e1 x e')
+          | e_if e0 e1 e2 => e_if (sbst' e0 x e') (sbst' e1 x e') (sbst' e2 x e')
+          | _ => e
+          end
+    }.
+
+  #[global] Instance asrt_subst : Subst asrt var exp:=
+    {
+      sbst :=
+        fix sbst' A x e :=
+          match A with
+          | a_exp e' => a_exp ([e /s x] e')
+
+          | A1 ∧ A2 => (sbst' A1 x e) ∧ (sbst' A2 x e)
+          | A1 ∨ A2 => (sbst' A1 x e) ∨ (sbst' A2 x e)
+          | ¬ A' => ¬ (sbst' A' x e)
+          | a_all A' => a_all (sbst' A' x e)
+          | a_ex A' => a_ex (sbst' A' x e)
+
+          | a_intl e' => a_intl ([e /s x] e')
+          | a_extl e' => a_extl ([e /s x] e')
+
+          | a_prt e' => a_prt ([e /s x] e')
+          | a_prt_frm e1 e2 => a_prt_frm ([e /s x] e1) ([e /s x] e2)
+          end
+    }.
+
+  Notation "e ∙ f" := (e_fld e f)(at level 38).
+  Notation "'e_' x" := (e_var x)(at level 38).
+  Notation "'a_' e" := (a_exp e)(at level 38).
+  Notation "e1 ⩵ e2" := (e_eq e1 e2)(at level 38).
+
+  Inductive hoare : module -> asrt -> stmt -> asrt -> Prop :=
+  | h_class : forall M e C s, hoare M (a_ e_class e C) s (a_ e_class e C)
+
+  | h_intl : forall M e s, hoare M (a_intl e) s (a_intl e)
+
+  | h_extl : forall M e s, hoare M (a_extl e) s (a_extl e)
+
+  | h_read : forall M x y f P, hoare M ([e_ y∙f /s x] P) (s_read x y f) P
+
+  | h_write1 : forall M x f y P, hoare M P (s_write x f y) (a_ e_ x∙f ⩵ e_ y)
+
+  | h_strengthen : forall M s P1 P2 Q, hoare M P1 s Q ->
+                                  asrt_proof M (P2 ⟶ P1) ->
+                                  hoare M P2 s Q
+
+  | h_weaken : forall M s P Q1 Q2, hoare M P s Q1 ->
+                              asrt_proof M (Q1 ⟶ Q2) ->
+                              hoare M P s Q2
+
+  | h_if : forall M e s1 s2 P Q, hoare M (P ∧ a_ e) s1 Q ->
+                            hoare M (P ∧ ¬ a_ e) s2 Q ->
+                            hoare M P (s_if e s1 s2) Q.
 
 End Hoare.
